Experiments/ProofChecking/SRChecker.lean
@@ -1,696 +1,368 @@
 /-
 
-Theory and implementation for the SR proof system and a checker.
+An LSR proof checker, with proof of correctness.
 
-Authors: Cayden Codel
+Uses `RangeArray`s to efficiently implement CNF formulas with deletion.
+
+Author: Cayden Codel
 Carnegie Mellon University
 
 -/
 
+import Experiments.ProofChecking.RangeArray
+import Experiments.ProofChecking.SRParser
 import Experiments.ProofChecking.PPA
 import Experiments.ProofChecking.PS
-import Experiments.ProofChecking.RangeArray
 
-import LeanSAT.Data.Cnf
-import LeanSAT.Data.ICnf
-import LeanSAT.Model.PropFun
-import LeanSAT.Model.Subst
+import LeanColls
+open LeanColls
 
-open LeanSAT LeanSAT.Model Nat
-open PPA PS LitVar ILit IVar LawfulLitVar PropFun
+open RangeArray
+open LeanSAT LeanSAT.Model
+open PPA PS
 open Except
 
-namespace PPA
+namespace RangeArray
 
-/-
-def unitPropFlat (τ : PPA) (F : RangeArray ILit) (i : Nat) : MUPResult :=
-  match F.foldlM_index (pevalUP τ) none i with
-  | ok none => .falsified
-  | ok (some lit) => .unit lit
-  | error true => .satisfied
-  | error false => .multipleUnassignedLiterals -/
 
--- TODO: Some correctness theorem relating this to unitProp
+def uAssumeNegatedForM (F : RangeArray ILit) (τ : PPA) (bumps : Nat) : Except PPA PPA :=
+  let usize := F.usize
+  let rec loop (i : Nat) (τ : PPA) : Except PPA PPA :=
+    if h : i < usize then
+      let l := F.ugetFin ⟨i, h⟩
+      match τ.litValue? l with
+      | none       => loop (i + 1) (τ.setLitFor (-l) bumps)
+      | some false => loop (i + 1) τ
+      | some true  => .error τ
+    else
+      .ok τ
+  termination_by F.usize - i
+  loop 0 τ
 
-end PPA
+def uAssumeNegatedFor (F : RangeArray ILit) (τ : PPA) (bumps : Nat) : PPA × Bool :=
+  let usize := F.usize
+  let rec loop (i : Nat) (τ : PPA) : (PPA × Bool) :=
+    if h : i < usize then
+      let l := F.ugetFin ⟨i, h⟩
+      match τ.litValue? l with
+      | none       => loop (i + 1) (τ.setLitFor (-l) bumps)
+      | some false => loop (i + 1) τ
+      | some true  => (τ, true)
+    else
+      (τ, false)
+  termination_by F.usize - i
+  loop 0 τ
 
-namespace PS
-
-/-
-def seval (σ : PS) (p : Bool × Bool) (l : ILit) : Except Unit (Bool × Bool) :=
-  -- Has there been a non-id map, and has there been a literal that's unassigned
-  let ⟨reduced?, unassigned?⟩ := p
-  match σ.litValue l with
-  | .tr => error ()
-  | .fls => ok (true, unassigned?)
-  | .lit lit => ok (reduced? || (l != lit), true) -/
-
-/-
-def reduceFlat (σ : PS) (F : RangeArray ILit) (i : Nat) : ReductionResult :=
-  match F.foldlM_index (seval σ) false i with
-  | ok true => .reduced
-  | ok false => .notReduced
-  | error _ => .satisfied
--/
--- TODO: Some correctness theorem releating this to reduce
-
-end PS
-
-namespace SR
-
-inductive UPResult
-  | checked : UPResult
-  | checkError : UPResult
-
-open UPResult
-
-structure SRLine where
-  clause : IClause
-  witness_lits : Array ILit
-  witness_maps : Array (IVar × ILit)
-  up_hints : Array Nat                -- Already 0-indexed clause IDs into the accumulated formula
-  rat_hints : Array (Nat × Array Nat) -- Already 0-indexed clause IDs into the accumulated formula
-
-structure SRState where
-  F : ICnf -- Accumulated formula
-  τ : PPA  -- Partial assignment, to store candidate and RAT negations
-  σ : PS   -- Substitution, for the witness
-
--- Applies a single unit propagation step
--- On success, we set the unit literal in τ with the offset
--- On falsification of the clause, we error with .checked
--- On satisfied clause or multiple unassigned literals, we error with checkError
-def applyUPHint (F : ICnf) (offset : Nat) (τ : PPA) (hint : Nat) : Except (PPA × UPResult) PPA :=
-  if h_hint : hint < F.size then
-    let C := F.get ⟨hint, h_hint⟩
-    match τ.unitProp C with
-    | .falsified => error ⟨τ, .checked⟩
-    | .satisfied =>
-      --dbg_trace s!"ERROR: UP found a satisfied clause"
-      error ⟨τ, .checkError⟩
-    | .multipleUnassignedLiterals =>
-      --dbg_trace s!"ERROR: UP found a non-unit clause"
-      error ⟨τ, .checkError⟩
-    | .unit l => ok (τ.setLitFor l offset)
-  else
-    --dbg_trace s!"ERROR: Hint out of bounds"
-    error ⟨τ, .checkError⟩
-
-def scanRATHints (clauseId : Nat) (ratHints : Array (Nat × Array Nat)) : Option (Fin ratHints.size) :=
-  match ratHints.foldlM (init := 0) (fun counter ⟨hint, _⟩ =>
-        if hint = clauseId then error counter
-        else ok (counter + 1)) with
-  | ok _ => none
-  | error index =>
-    if hi : index < ratHints.size then some ⟨index, hi⟩
-    else none
-
--- Finds the RAT hint pair that matches the clauseId
-def findRATHintIndex (ratIndex clauseId : Nat) (ratHints : Array (Nat × Array Nat)) : Option (Fin ratHints.size) :=
-  -- If the RAT hints are sorted, then check the one under our "cached pointer" first
-  if h_index : ratIndex < ratHints.size then
-    let ⟨ratClauseIndex, _⟩ := ratHints.get ⟨ratIndex, h_index⟩
-    if ratClauseIndex = clauseId then some ⟨ratIndex, h_index⟩
-    else scanRATHints clauseId ratHints
-  else
-    scanRATHints clauseId ratHints
-
--- Assuming that (C|σ) is reduced but not satisfied and that C is a RAT clause, sets τ ← τ ⊓ (C|σ)ᶜ
-def assumeRATClause (C : IClause) (σ : PS) (τ : PPA) : Except PPA PPA :=
-  C.foldlM (init := τ) (fun τ lit =>
+-- TODO: Swap with tail-recursive function, move to PS.
+/-- Assumes into `τ` the negation of RAT clause `C` under the substitution `σ` for one "bump."
+    Errors if `C` is satisfied by either `σ` or `τ` under `σ`. -/
+def assumeRATClauseM (F : RangeArray ILit) (index : Fin F.size) (σ : PS) (τ : PPA) : Except PPA PPA :=
+  F.foldlM_index (init := τ) (fun τ lit =>
     match σ.litValue lit with
     | Sum.inr true => error τ       -- (C|σ) is satisfied, so return early to report satisfied
     | Sum.inr false => ok τ         -- Ignore the literal
     | Sum.inl l =>
       match τ.litValue? l with
-      | some true => error τ    -- (C|σ)|τ is satisfied, so return early to report satisfied
-      | some false => ok τ      -- Its negation is true in τ, so ignore the literal
-      | none => ok (τ.setLit (-l)))
+      | some true => error τ        -- (C|σ)|τ is satisfied, so return early to report satisfied
+      | some false => ok τ          -- Its negation is true in τ, so ignore the literal
+      | none => ok (τ.setLit (-l))) index
 
--- Set the witness substitution σ from the provided mapping, resetting σ first
-def assumeWitness (σ : PS) (pivot : ILit) (A₁ : Array ILit) (A₂ : Array (IVar × ILit)) : PS :=
-  ((σ.reset.setLits A₁).setVars A₂).setLit pivot
+def assumeRATClause (F : RangeArray ILit) (index : Fin F.size) (σ : PS) (τ : PPA) : PPA × Bool :=
+  let rsize := F.rsizeFin index
+  let rec loop (i : Nat) (τ : PPA) : PPA × Bool :=
+    if h : i < rsize then
+      let lit := F.ogetFin index ⟨i, h⟩
+      match σ.litValue lit with
+      | Sum.inr true => ⟨τ, true⟩
+      | Sum.inr false => loop (i + 1) τ
+      | Sum.inl l =>
+        match τ.litValue? l with
+        | some true => ⟨τ, true⟩
+        | some false => loop (i + 1) τ
+        | none => loop (i + 1) (τ.setLit (-l))
+    else
+      ⟨τ, false⟩
+  termination_by F.rsizeFin index - i
+  loop 0 τ
 
--- Check each clause in the formula.
--- C is the current clause in the formula to be checked for the RAT property under σ and τ
--- If C is reduced by σ, then it is RAT. Find a RAT hint and uses the RAT UP hints to derive contradiction.
-def checkClause (F : ICnf) (σ : PS) (ratHints : Array (Nat × Array Nat))
-    (p : PPA × Nat × Nat × Nat) (C : IClause) : Except Unit (PPA × Nat × Nat × Nat) :=
-  let ⟨τ, ratIndex, index, bumpCounter⟩ := p
-  --let F := dbgTraceIfShared "Formula in checkClause" F
-  match σ.seval_fold C with
-  | .satisfied => ok (τ, ratIndex, index + 1, bumpCounter)
-  | .notReduced => ok (τ, ratIndex, index + 1, bumpCounter)
-  | _ =>
-    -- We expect a RAT clause. Check if we have bumps left
-    if bumpCounter < ratHints.size then
-      -- Curiously, if the clause is completely falsified, we can still succeed
-      -- on the check (which sr-check does not allow). This is because a UP
-      -- derivation on a completely falsified clause is a global UP derivation,
-      -- and so the certificate can be reduced quite a bit.
-
-      -- Find a RAT hint matching the clause
-      -- We hope that the hints are sorted, but they don't have to be
-      match findRATHintIndex ratIndex index ratHints with
-      | none => error ()
-      | some rI =>
-        let ⟨_, hints⟩ := ratHints.get rI
-        match assumeRATClause C σ τ with
-        -- If the clause is satisfied under σ and τ, then we move to the next iteration
-        | error τ => ok (τ.bump, rI.val + 1, index + 1, bumpCounter + 1)
-
-        -- Otherwise, we have assumed the negation of the RAT clause
-        -- Now check for UP derivation through its hints
-        | ok τ =>
-          match hints.foldlM (init := τ) (applyUPHint F 0) with
-          | error (τ, .checked) => ok (τ.bump, rI.val + 1, index + 1, bumpCounter + 1)
-          | error (_, .checkError) => error ()
-          | ok _ => error ()
-    -- We error if the bumpCounter equals the number of RAT hints, since that
-    -- means we bumped the assignment too many times, clearing out the
-    -- assumption of the candidate clause
-    else error ()
-
-
-def checkLine (S : SRState) (line : SRLine) : Except Bool SRState :=
-  let ⟨F, τ, σ⟩ := dbgTraceIfShared "Formula at start of checkLine" S
-  let ⟨C, w_tf, w_maps, UPhints, RAThints⟩ := line
-
-  -- Assumes the negation of the candidate clause, with "# of RAT hints" offset
-  match assumeNegatedClauseFor τ.reset C (RAThints.size + 1) with
-  | error _ => error false
-  | ok τ =>
-
-  -- Evaluate the UP hints, with "# of RAT hints" offset
-  -- We add one more than normal to help with proving
-  match UPhints.foldlM (init := τ) (applyUPHint F (RAThints.size + 1)) with
-  -- The clause led to contradiction via unit propagation
-  | error ⟨τ, .checked⟩ =>
-    if C = #[] then error true       -- If the clause is empty, we have a successful proof
-    else ok ⟨F.addClause C, τ, σ⟩ -- The clause is redundant, so add it to the formula
-
-  -- Unit propagation failed due to multiple unassigned literals, satisfied clause, or out-of-bounds
-  | error ⟨_, _⟩ => error false
-
-  -- Unit propagation worked but didn't lead to contradiction, so continue to RAT checking
-  | ok τ =>
-
-    -- If the clause is empty, then we should have derived UP contradiction by now
-    if hCw : 0 < C.size ∧ 0 < w_tf.size then
-      if C.get ⟨0, hCw.1⟩ ≠ w_tf.get ⟨0, hCw.2⟩ then error false else
-
-      -- Assume the witness, under substitution (the function call resets σ)
-      let σ := assumeWitness σ (C.get ⟨0, hCw.1⟩) w_tf w_maps
-      let F := dbgTraceIfShared "Formula" F
-
-      -- Go through each clause in the formula to check RAT
-      match F.foldlM (init := (⟨τ, 0, 0, 0⟩ : PPA × Nat × Nat × Nat)) (checkClause F σ RAThints) with
-      | error () => error false
-      | ok (τ, _) =>
-        --let F := dbgTraceIfShared "Formula at end of checkLine" F
-        ok ⟨F.addClause C, τ, σ⟩ -- The RAT hint checked, so we continue
-
-    else error false
-
-def checkProof (F : ICnf) (proof : Array SRLine) : Bool :=
-  let τ := PPA.new 100
-  let σ := PS.new 100
-  match proof.foldlM (init := ⟨F, τ, σ⟩) checkLine with
-  | ok _ => false
-  | error false => false
-  | error true => true
-
-/-! # flat version -/
-
-/-
-structure FlatState where
-  formula : RangeArray ILit -- Accumulated formula
-  τ : PPA                   -- Partial assignment, to store candidate and RAT negations
-  σ : PS                    -- Substitution, for the witness
-
-
-
--- Applies a single unit propagation step
--- On success, we set the unit literal in τ with the offset
--- On falsification of the clause, we error with .checked
--- On satisfied clause or multiple unassigned literals, we error with checkError
-def applyUPHintFlat (F : RangeArray ILit) (offset : Nat) (τ : PPA) (hint : Nat) : Except (PPA × UPResult) PPA :=
-  if hint < F.size then
-    match τ.unitPropFlat F hint with
-    | .falsified => error ⟨τ, .checked⟩
-    | .satisfied =>
-      --dbg_trace s!"ERROR: UP found a satisfied clause"
-      error ⟨τ, .checkError⟩
-    | .multipleUnassignedLiterals =>
-      --dbg_trace s!"ERROR: UP found a non-unit clause"
-      error ⟨τ, .checkError⟩
-    | .unit l =>
-      --dbg_trace s!"    Hint {hint} makes clause unit on literal {l}"
-      ok (τ.setLitFor l offset)
-  else
-    --dbg_trace s!"ERROR: Hint out of bounds"
-    error ⟨τ, .checkError⟩
-
--- Assuming that (C|σ) is reduced but not satisfied and that C is a RAT clause, sets τ ← τ ⊓ (C|σ)ᶜ
-def assumeRATClauseFlat (F : RangeArray ILit) (i : Nat) (σ : PS) (τ : PPA) : Except PPA PPA :=
-  F.foldlM_index (i := i) (init := τ) (fun τ lit =>
-    match σ.litValue lit with
-    | .tr => error τ       -- (C|σ) is satisfied, so return early to report satisfied
-    | .fls => ok τ         -- Ignore the literal
-    | .lit l =>
-      match τ.litValue? l with
-      | some true => error τ    -- (C|σ)|τ is satisfied, so return early to report satisfied
-      | some false => ok τ      -- Its negation is true in τ, so ignore the literal
-      | none => ok (τ.setLit (-l)))
-
--- Check each clause in the formula.
--- C is the current clause in the formula to be checked for the RAT property under σ and τ
--- If C is reduced by σ, then it is RAT. Find a RAT hint and uses the RAT UP hints to derive contradiction.
-def checkClauseFlat (F : RangeArray ILit) (σ : PS) (ratHints : Array (Nat × Array Nat))
-    (p : PPA × Nat × Nat) (i : Nat) : Except Unit (PPA × Nat × Nat) :=
-  let ⟨τ, ratIndex, bumpCounter⟩ := p
-  match σ.reduceFlat F i with
-  | .satisfied => ok (τ, ratIndex, bumpCounter)
-  | .notReduced => ok (τ, ratIndex, bumpCounter)
-  | _ =>
-    --dbg_trace s!"     Clause {i} is reduced, checking for RAT"
-    -- We expect a RAT clause. Check if we have bumps left
-    if bumpCounter < ratHints.size then
-      -- Curiously, if the clause is completely falsified, we can still succeed
-      -- on the check (which sr-check does not allow). This is because a UP
-      -- derivation on a completely falsified clause is a global UP derivation,
-      -- and so the certificate can be reduced quite a bit.
-
-      -- Find a RAT hint matching the clause (add one to the current index, due to 1-indexing)
-      -- We hope that the hints are sorted, but they don't have to be
-      match findRATHintIndex ratIndex i ratHints with
+def unitProp (τ : PPA) (F : RangeArray ILit) (hint : Fin F.size) : PPA.UPResult :=
+  let rsize := F.rsizeFin hint
+  let rec loop (i : Nat) (unit? : Option ILit) : PPA.UPResult :=
+    if hi : i < rsize then
+      let lit := F.ogetFin hint ⟨i, hi⟩
+      match τ.litValue? lit with
+      | some true => .satisfied
+      | some false => loop (i + 1) unit?
       | none =>
-        --dbg_trace s!"Clause {i} found to be missing a RAT hint"
-        error ()
-      | some rI =>
-        let ⟨_, hints⟩ := ratHints.get rI
-        match assumeRATClauseFlat F i σ τ with
-        -- If the clause is satisfied under σ and τ, then we move to the next iteration
-        | error τ => ok (τ.bump, rI.val + 1, bumpCounter + 1)
-
-        -- Otherwise, we have assumed the negation of the RAT clause
-        -- Now check for UP derivation through its hints
-        | ok τ =>
-          match hints.foldlM (init := τ) (applyUPHintFlat F 0) with
-          | error (τ, .checked) => ok (τ.bump, rI.val + 1, bumpCounter + 1)
-          | error (_, .checkError) =>
-            --dbg_trace s!"ERROR: UP failed"
-            error ()
-          | ok _ =>
-            --dbg_trace s!"ERROR: UP succeeded, but didn't lead to contradiction"
-            error ()
-    -- We error if the bumpCounter equals the number of RAT hints, since that
-    -- means we bumped the assignment too many times, clearing out the
-    -- assumption of the candidate clause
+        match unit? with
+        | none => loop (i + 1) (some lit)
+        | some u =>
+          if u = lit then loop (i + 1) unit?
+          else .multipleUnassignedLiterals
     else
-      --dbg_trace s!"ERROR: Bump counter exceeded number of RAT hints"
-      error ()
+      match unit? with
+      | none => .falsified
+      | some l => .unit l
+  termination_by F.rsizeFin hint - i
+  loop 0 none
 
-def checkLineFlat (S : FlatState) (line : SRLine) : Except Bool FlatState :=
-  --dbg_trace s!"About to check line with clause {line.clause}"
-  let ⟨F, τ, σ⟩ := S
-  let ⟨C, w_tf, w_maps, UPhints, RAThints⟩ := line
+inductive HintResult where
+  | unit
+  | contra
+  | err
+  deriving DecidableEq, Inhabited
 
-  -- Assumes the negation of the candidate clause, with "# of RAT hints" offset
-  match assumeNegatedClauseFor τ.reset C (RAThints.size + 1) with
+@[inline]
+def applyUPHint (F : RangeArray ILit) (bumps : Nat) (τ : PPA) (hint : Nat) : PPA × HintResult :=
+  if h_hint : hint < F.size then
+    if !F.isDeleted hint then
+      match unitProp τ F ⟨hint, h_hint⟩ with
+      | .falsified => ⟨τ, .contra⟩
+      | .satisfied =>
+        -- dbg_trace s!"ERROR: UP found a satisfied clause at index {hint}"
+        ⟨τ, .err⟩
+      | .multipleUnassignedLiterals =>
+        -- dbg_trace s!"ERROR: UP found a non-unit clause at index {hint}"
+        ⟨τ, .err⟩
+      | .unit l =>
+        -- dbg_trace s!"    Hint {hint} makes clause unit on literal {l}"
+        (τ.setLitFor l bumps, .unit)
+    else
+      ⟨τ, .err⟩
+  else
+    -- dbg_trace s!"ERROR: Hint out of bounds"
+    ⟨τ, .err⟩
+
+@[inline, always_inline]
+def applyUPHints (F : RangeArray ILit) (offset : Nat) (τ : PPA) (hints : Array Nat) : PPA × HintResult :=
+  let rec loop (i : Nat) (τ : PPA) : PPA × HintResult :=
+    if hi : i < Size.size hints then
+      match applyUPHint F offset τ (Seq.get hints ⟨i, hi⟩) with
+      | (τ, .unit) => loop (i + 1) τ
+      | (τ, .contra) => (τ, .contra)
+      | (τ, .err) => (τ, .err)
+    else (τ, .unit)
+  termination_by hints.size - i
+  loop 0 τ
+
+def reduce (σ : PS) (F : RangeArray ILit) (index : Fin F.size) : ReductionResult :=
+  let rsize := F.rsizeFin index
+  let rec loop (i : Nat) (reduced? : Bool) : ReductionResult :=
+    if hi : i < rsize then
+      let lit := F.ogetFin index ⟨i, hi⟩
+      match seval' σ lit with
+      | .satisfied => .satisfied
+      | .reduced => loop (i + 1) true
+      | .notReduced => loop (i + 1) reduced?
+    else
+      if reduced? then .reduced else .notReduced
+  termination_by F.rsizeFin index - i
+  loop 0 false
+
+def reduce' (σ : PS) (F : RangeArray ILit) (index : Fin F.size) : ReductionResult :=
+  let rsize := F.rsizeFin index
+  let rstart := F.indexFin index
+  let rec loop (i : Nat) (reduced? : Bool) : ReductionResult :=
+    if hi : i < rsize then
+      let lit := F.getFin ⟨rstart + i, index_add_offset_in_range index ⟨i, hi⟩⟩
+      match seval' σ lit with
+      | .satisfied => .satisfied
+      | .reduced => loop (i + 1) true
+      | .notReduced => loop (i + 1) reduced?
+    else
+      if reduced? then .reduced else .notReduced
+  termination_by F.rsizeFin index - i
+  loop 0 false
+
+-- CC: Causes quadratic(?) slowdown, from 0.79 secs to 12.21 secs on php25
+--     Profiler claims that 41% of CPU is spent in σ.setLits though...
+def reduceM (σ : PS) (F : RangeArray ILit) (index : Fin F.size)
+    (h_del : F.isDeletedFin index = false) : ReductionResult :=
+  match ((F.foldlM_indexHyps (fun reduced? lit =>
+    match seval' σ lit with
+    | .satisfied => throw ()
+    | .reduced => return true
+    | .notReduced => return reduced?) false index h_del) : Except Unit Bool) with
+  | .ok reduced? => if reduced? then .reduced else .notReduced
+  | .error _ => .satisfied
+
+end RangeArray
+
+namespace SR
+
+-- Scans through the RAT hint clause IDs to find a matching ID
+def scanRATHintIndexesM (clauseId : Nat) (ratHintIndexes : Array Nat) : Option (Fin ratHintIndexes.size) :=
+  match ratHintIndexes.foldlM (init := 0) (fun counter hint =>
+        if hint = clauseId then error counter
+        else ok (counter + 1)) with
+  | ok _ => none
+  | error index =>
+    if hi : index < Size.size ratHintIndexes then
+      some ⟨index, hi⟩
+    else
+      none
+
+def scanRATHintIndexes (clauseId : Nat) (ratHintIndexes : Array Nat) : Option (Fin ratHintIndexes.size) :=
+  let rec loop (i : Nat) : Option (Fin ratHintIndexes.size) :=
+    if h : i < Size.size ratHintIndexes then
+      if Seq.get ratHintIndexes ⟨i, h⟩ = clauseId then some ⟨i, h⟩
+      else loop (i + 1)
+    else none
+  termination_by ratHintIndexes.size - i
+  loop 0
+
+-- Finds the index for the (RAT clause ID + RAT hints) that matches the clauseId
+def findRATHintIndex (ratIndex clauseId : Nat) (ratHintIndexes : Array Nat) : Option (Fin ratHintIndexes.size) :=
+  -- If the RAT hints are sorted, then check the one under our "cached pointer" first
+  if h_index : ratIndex < Size.size ratHintIndexes then
+    let ratClauseIndex := Seq.get ratHintIndexes ⟨ratIndex, h_index⟩
+    if ratClauseIndex = clauseId then
+      some ⟨ratIndex, h_index⟩
+    else
+      -- TODO: Test with `M` here.
+      scanRATHintIndexes clauseId ratHintIndexes
+  else
+    scanRATHintIndexes clauseId ratHintIndexes
+
+
+/-- Set the witness substitution σ from the provided mapping, resetting σ first. -/
+def assumeWitness (σ : PS) (pivot : ILit) (A₁ : Array ILit) (A₂ : Array ILit) : PS :=
+  ((σ.reset.setLits A₁).setVars' A₂).setLit pivot
+
+structure SRState where
+  F : RangeArray ILit
+  τ : PPA
+  σ : PS
+
+def checkLine (st : SRState) (line : SRAdditionLine) : Except Bool SRState :=
+  --let ⟨C, wL, wM, upHints, ratHintIndexes, ratHints, _, _⟩ := line
+  -- dbg_trace s!"{C}, {wL}, {wM}"
+  -- dbg_trace s!"{upHints}, {ratHintIndexes}, {ratHints}"
+  match uAssumeNegatedForM st.F st.τ.reset (line.ratHints.size + 1) with
   | error _ =>
-    --dbg_trace s!"ERROR: Assumption of clause failed"
+    -- dbg_trace s!"Assuming the negation of the candidate clause had error"
     error false
   | ok τ =>
-
-  --dbg_trace s!"Assumed negation of {C} with {RAThints.size + 1} offset"
-
-  -- Evaluate the UP hints, with "# of RAT hints" offset
-  -- We add one more than normal to help with proving
-  match UPhints.foldlM (init := τ) (applyUPHintFlat F (RAThints.size + 1)) with
-  -- The clause led to contradiction via unit propagation
-  | error ⟨τ, .checked⟩ =>
-    if C = #[] then error true       -- If the clause is empty, we have a successful proof
-    else ok ⟨F.add C, τ, σ⟩ -- The clause is redundant, so add it to the formula
-
-  -- Unit propagation failed due to multiple unassigned literals, satisfied clause, or out-of-bounds
-  | error ⟨_, _⟩ =>
-    --dbg_trace s!"ERROR: UP failed"
-    error false
-
-  -- Unit propagation worked but didn't lead to contradiction, so continue to RAT checking
-  | ok τ =>
-
-    --dbg_trace s!"  UP succeeded, checking for RAT"
-
-    -- If the clause is empty, then we should have derived UP contradiction by now
-    if hCw : 0 < C.size ∧ 0 < w_tf.size then
-      if C.get ⟨0, hCw.1⟩ ≠ w_tf.get ⟨0, hCw.2⟩ then
-        --dbg_trace s!"Pivot doesn't agree with 0th literal"
-        error false
-      else
-
-      -- Assume the witness, under substitution (the function call resets σ)
-      let σ := assumeWitness σ (C.get ⟨0, hCw.1⟩) w_tf w_maps
-
-      -- Go through each clause in the formula to check RAT
-      match F.foldlM_over_indexes (init := (⟨τ, 0, 0⟩ : PPA × Nat × Nat)) (checkClauseFlat F σ RAThints) with
-      | error () =>
-        --dbg_trace s!"ERROR: RAT check failed"
-        error false
-      | ok (τ, _) =>
-        --dbg_trace s!"RAT check succeeded, adding clause {C}"
-        ok ⟨F.add C, τ, σ⟩ -- The RAT hint checked, so we continue
-
-    else
-      --dbg_trace s!"ERROR: Either the clause or the true/false mappings are empty"
+    let st := { st with τ := τ }
+    -- dbg_trace s!"Assumed negation of clause succeeded"
+    -- Evaluate the UP hints, with "# of RAT hints" as the offset
+    match applyUPHints st.F (line.ratHints.size + 1) st.τ line.upHints with
+    | (_, .err) =>
+      -- dbg_trace s!"Applying UP hints encountered an error"
       error false
+    | (τ, .contra) =>
+      let st := { st with τ := τ }
+      -- dbg_trace s!"Applying UP hints found contradiction before RAT"
+      if st.F.usize = 0 then error true  -- If the clause is empty, we have a successful contradiction proof
+      else ok { st with F := st.F.commit }
 
-#exit
--/
+    | (τ, .unit) =>
+      let st := { st with τ := τ }
 
-/-! # correctness -/
+      -- If the clause is empty, we should have derived UP contradiction by now
+      if hu : 0 < st.F.usize then
+        let pivot : ILit := line.witnessLits.getD 0 (st.F.ugetFin ⟨0, hu⟩)
+        if pivot != st.F.ugetFin ⟨0, hu⟩ then error false else
+        let st := { st with σ := assumeWitness st.σ pivot line.witnessLits line.witnessMaps }
 
--- TODO: Exists a PS, or forall PS that meet the condition?
--- TODO: Can be "generalized" to one for (IVar → PropForm IVar), or maybe just substitutions in general
-theorem SR_core {F : ICnf} {C : IClause} {σ : PS} :
-    PropFun.substL C σ.toSubst = ⊤ → F.toPropFun ⊓ Cᶜ ≤ PropFun.substL F σ.toSubst →
-    eqsat F (F ⊓ C.toPropFun) := by
-  intro hC hFC
-  constructor
-  · rintro ⟨τ, hτF⟩
-    by_cases hτC : τ ⊨ C.toPropFun
-    · use τ
-      rw [satisfies_conj]
-      exact ⟨hτF, hτC⟩
-    · replace hFC := entails_ext.mp hFC τ
-      simp [satisfies_conj, and_imp, -satisfies_substL] at hFC
-      replace hFC := hFC hτF hτC
-      have : τ ⊨ PropFun.substL C σ.toSubst := by rw [hC]; rfl
-      simp at hFC this
-      use PropAssignment.subst (fun x => ⟦σ.toSubst x⟧) τ
-      rw [satisfies_conj]
-      exact ⟨hFC, this⟩
-  · rintro ⟨τ, hτ⟩
-    rw [satisfies_conj] at hτ
-    exact ⟨τ, hτ.1⟩
+        -- Loop through each clause in the formula to check RAT conditions
+        -- The Bool is true if the check succeeds on all clauses, false otherwise
+        let Fsize := st.F.size
+        let rec loop (i cachedRatHintIndex bumpCounter : Nat) (τ : PPA) : PPA × Bool :=
+          if hi : i < Fsize then
+            if h_del : st.F.isDeletedFin ⟨i, hi⟩ = true then
+              loop (i + 1) cachedRatHintIndex bumpCounter τ
+            else
+              -- First, check how the ith clause is reduced by σ
+              match reduce st.σ st.F ⟨i, hi⟩ with
+              | .satisfied => loop (i + 1) cachedRatHintIndex bumpCounter τ
+              | .notReduced => loop (i + 1) cachedRatHintIndex bumpCounter τ
+              | _ =>
+                -- dbg_trace s!"Clause index {i} is a RAT candidate"
+                if bumpCounter < line.ratHintIndexes.size then
+                  -- Find the corresponding RAT hint
+                  match findRATHintIndex cachedRatHintIndex i line.ratHintIndexes with
+                  | none => ⟨τ, false⟩
+                  | some ⟨ratIndex, hr⟩ =>
+                    -- Assume the negation of the RAT clause
+                    match assumeRATClause st.F ⟨i, hi⟩ st.σ τ with
+                    | ⟨τ, true⟩ => loop (i + 1) (ratIndex + 1) (bumpCounter + 1) τ.bump
+                    | ⟨τ, false⟩ =>
+                      match applyUPHints st.F 0 τ (line.ratHints.get ⟨ratIndex, by rw [line.ratSizesEq] at hr; exact hr⟩) with
+                      | (τ, .unit) => ⟨τ, false⟩
+                      | (τ, .contra) => loop (i + 1) (ratIndex + 1) (bumpCounter + 1) τ.bump
+                      | (τ, .err) => ⟨τ, false⟩
+                else ⟨τ, false⟩
+          else ⟨τ, true⟩
+        termination_by st.F.size - i
 
-theorem assumeWitness_subst {C : IClause} (hC : 0 < C.size) :
-      ∀ σ A₁ A₂, PropFun.substL C.toPropFun (assumeWitness σ (C.get ⟨0, hC⟩) A₁ A₂).toSubst = ⊤ := by
-  intro σ A₁ A₂
-  rw [assumeWitness]
-  simp [PropFun.ext_iff]
-  intro τ
-  rw [Clause.satisfies_iff]
-  use C.get ⟨0, hC⟩
-  constructor
-  · simp [← Array.mem_data]; exact Array.getElem_mem_data C hC
-  · simp [LitVar.satisfies_iff, PropAssignment.subst]
-    sorry
-  done
+        match loop 0 0 0 st.τ with
+        | ⟨_, false⟩ => error false
+        | ⟨τ, true⟩ => ok { st with τ := τ, F := st.F.commit }
+      else error false
 
--- TODO: Is the standard `≤ ⊥` or `= ⊥`?
-theorem applyUPHint_checked {F : ICnf} {offset : Nat} {τ τ' : PPA} {hint : Nat} :
-    applyUPHint F offset τ hint = .error (τ', .checked) →
-      τ = τ' ∧ F.toPropFun ⊓ τ ≤ ⊥ := by
-  rw [applyUPHint]
-  split <;> simp
-  split <;> simp
-  rintro rfl; use rfl
-  rename hint < F.size => h_hint
-  rename (unitProp τ _ = _) => h_up
-  have := contradiction_of_UP_falsified h_up
-  rw [inf_comm] at this
-  rw [← le_bot_iff]
-  exact le_trans (inf_le_inf_right τ.toPropFun (Cnf.ith_le ⟨hint, h_hint⟩)) this
+/-def checkLine (F : RangeArray ILit) (τ : PPA) (σ : PS) (line : SRAdditionLine)
+    : Except Bool (RangeArray ILit × PPA × PS) :=
+  --let ⟨C, wL, wM, upHints, ratHintIndexes, ratHints, _, _⟩ := line
+  -- dbg_trace s!"{C}, {wL}, {wM}"
+  -- dbg_trace s!"{upHints}, {ratHintIndexes}, {ratHints}"
+  match uAssumeNegatedForM F τ.reset (line.ratHints.size + 1) with
+  | error _ =>
+    -- dbg_trace s!"Assuming the negation of the candidate clause had error"
+    error false
+  | ok τ =>
+    -- dbg_trace s!"Assumed negation of clause succeeded"
+    -- Evaluate the UP hints, with "# of RAT hints" as the offset
+    match applyUPHints F (line.ratHints.size + 1) τ line.upHints with
+    | (_, .err) =>
+      -- dbg_trace s!"Applying UP hints encountered an error"
+      error false
+    | (τ, .contra) =>
+      -- dbg_trace s!"Applying UP hints found contradiction before RAT"
+      if F.usize = 0 then error true  -- If the clause is empty, we have a successful contradiction proof
+      else ok ⟨F.commit, τ, σ⟩
 
--- TODO: Do we need everything in our spec?
--- Also, the spec is not strong enough to derive ge_of_applyUPHint_ok because
--- it doesn't comment on the state of F[hint]. See
-theorem applyUPHint_ok {F : ICnf} {offset : Nat} {τ τ' : PPA} {hint : Nat} :
-    applyUPHint F offset τ hint = .ok τ' →
-      --∃ l, l ∈ F[hint] ∧ τ.litValue? l = none ∧ τ' = τ.setLitFor l offset
-      ∃ l, τ.litValue? l = none ∧ τ' = τ.setLitFor l offset := by
-  rw [applyUPHint]
-  split <;> simp
-  split <;> simp
-  rename hint < F.size => h_hint
-  rename ILit => lit
-  rename (unitProp τ _ = _) => h_up
-  rintro rfl
-  rcases extended_of_UP_unit h_up with ⟨_, h₂, _⟩
-  exact ⟨lit, h₂, rfl⟩
+    | (τ, .unit) =>
+      -- If the clause is empty, we should have derived UP contradiction by now
+      if hu : 0 < F.usize then
+        let pivot : ILit := line.witnessLits.getD 0 (F.ugetFin ⟨0, hu⟩)
+        if pivot != F.ugetFin ⟨0, hu⟩ then error false else
+        let σ := assumeWitness σ pivot line.witnessLits line.witnessMaps
 
-theorem ge_of_applyUPHint_ok {F : ICnf} {offset : Nat} {τ τ' : PPA} {hint : Nat} :
-    applyUPHint F offset τ hint = .ok τ' → F.toPropFun ⊓ τ ≤ τ' := by
-  rw [applyUPHint]
-  split <;> simp
-  split <;> simp
-  rename hint < F.size => h_hint
-  rename ILit => lit
-  rename (unitProp τ _ = _) => h_up
-  rintro rfl
-  rcases extended_of_UP_unit h_up with ⟨_, h₂, h₃⟩
-  rw [toPropFun_setLitFor_eq_setLit, toPropFun_setLit_of_none h₂]
-  conv at h₃ => rhs; rw [inf_comm]
-  apply le_trans _ h₃
-  apply inf_le_inf_right
-  exact Cnf.ith_le ⟨hint, h_hint⟩
+        -- Loop through each clause in the formula to check RAT conditions
+        -- The Bool is true if the check succeeds on all clauses, false otherwise
+        let Fsize := F.size
+        let rec loop (i cachedRatHintIndex bumpCounter : Nat) (τ : PPA) : PPA × Bool :=
+          if hi : i < Fsize then
+            if h_del : F.isDeletedFin ⟨i, hi⟩ = true then
+              loop (i + 1) cachedRatHintIndex bumpCounter τ
+            else
+              -- First, check how the ith clause is reduced by σ
+              match reduce σ F ⟨i, hi⟩ with
+              | .satisfied => loop (i + 1) cachedRatHintIndex bumpCounter τ
+              | .notReduced => loop (i + 1) cachedRatHintIndex bumpCounter τ
+              | _ =>
+                -- dbg_trace s!"Clause index {i} is a RAT candidate"
+                if bumpCounter < line.ratHintIndexes.size then
+                  -- Find the corresponding RAT hint
+                  match findRATHintIndex cachedRatHintIndex i line.ratHintIndexes with
+                  | none => ⟨τ, false⟩
+                  | some ⟨ratIndex, hr⟩ =>
+                    -- Assume the negation of the RAT clause
+                    match assumeRATClause F ⟨i, hi⟩ σ τ with
+                    | ⟨τ, true⟩ => loop (i + 1) (ratIndex + 1) (bumpCounter + 1) τ.bump
+                    | ⟨τ, false⟩ =>
+                      match applyUPHints F 0 τ (line.ratHints.get ⟨ratIndex, by rw [line.ratSizesEq] at hr; exact hr⟩) with
+                      | (τ, .unit) => ⟨τ, false⟩
+                      | (τ, .contra) => loop (i + 1) (ratIndex + 1) (bumpCounter + 1) τ.bump
+                      | (τ, .err) => ⟨τ, false⟩
+                else ⟨τ, false⟩
+          else ⟨τ, true⟩
+        termination_by F.size - i
 
--- TODO: Package up τ = τ' invariants into "agreeOn" or "unchanged" or something
-theorem fold_UP_checked {F : ICnf} {A : Array Nat} {offset : Nat} {τ τ' : PPA} :
-    A.foldlM (init := τ) (applyUPHint F offset) = error (τ', .checked) →
-      F.toPropFun ⊓ τ ≤ ⊥ ∧ extended τ τ' offset := by
-  have ⟨A⟩ := A
-  rw [Array.foldlM_eq_foldlM_data]
-  induction' A with hint hints ih generalizing τ
-  · simp [pure, Except.pure]
-  · simp [-le_bot_iff]
-    intro h
-    match h_apply : applyUPHint F offset τ hint with
-    | error (τ₁, .checked) =>
-      rcases applyUPHint_checked h_apply with ⟨rfl, hτ⟩
-      use hτ
-      simp [h_apply] at h; injection h; rename _ => h
-      injection h; rename τ = τ' => heq; subst heq
-      simp [PPA.extended]
-      intro v hcon h
-      exact absurd h hcon
-    | error (τ₁, .checkError) =>
-      simp [h_apply] at h; injection h; rename _ => h
-      injection h
-      contradiction
-    | ok τ₁ =>
-      rcases applyUPHint_ok h_apply with ⟨l, hl, rfl⟩
-      -- TODO: What is a better hyp/spec?
-      have hFτ := ge_of_applyUPHint_ok h_apply
-      simp [h_apply] at h
-      rcases ih h with ⟨ih₁, ih₂⟩
-      rw [toPropFun_setLitFor_eq_setLit, toPropFun_setLit_of_none hl, ← inf_assoc] at ih₁
-      rw [toPropFun_setLitFor_eq_setLit, toPropFun_setLit_of_none hl] at hFτ
-      have := inf_le_inf_left F.toPropFun hFτ
-      simp_rw [← inf_assoc, inf_idem] at this
-      exact ⟨le_trans this ih₁, extended_trans (extended_setLitFor_of_none hl offset) ih₂⟩
-
-theorem fold_UP_ok {F : ICnf} {A : Array Nat} {offset : Nat} {τ τ' : PPA} :
-    A.foldlM (init := τ) (applyUPHint F offset) = ok τ' →
-      F.toPropFun ⊓ τ ≤ τ' ∧ extended τ τ' offset := by
-  have ⟨A⟩ := A
-  rw [Array.foldlM_eq_foldlM_data]
-  induction' A with hint hints ih generalizing τ
-  · simp [pure, Except.pure]; rintro rfl; exact ⟨inf_le_right, extended_refl _ _⟩
-  · simp
-    intro h
-    match h_apply : applyUPHint F offset τ hint with
-    | error _ => simp [h_apply] at h; injection h
-    | ok τ₁ =>
-      simp [h_apply] at h
-      rcases ih h with ⟨ih₁, ih₂⟩
-      rcases applyUPHint_ok h_apply with ⟨l, hl, rfl⟩
-      have := inf_le_inf_left F.toPropFun (ge_of_applyUPHint_ok h_apply)
-      rw [← inf_assoc, inf_idem] at this
-      exact ⟨le_trans this ih₁, extended_trans (extended_setLitFor_of_none hl offset) ih₂⟩
-
-theorem assumeRATClause_ok {C : IClause} {σ : PS} {τ τ' : PPA} :
-    assumeRATClause C σ τ = ok τ' →
-      τ.toPropFun ⊓ (PropFun.substL C σ.toSubst)ᶜ ≤ τ' ∧ extended τ τ' 0 := by
-  have ⟨C⟩ := C
-  rw [assumeRATClause, Array.foldlM_eq_foldlM_data]
-  induction' C with l ls ih generalizing τ
-  · simp [pure, Except.pure]; rintro rfl; exact ⟨le_refl _, extended_refl _ _⟩
-  · simp; split <;> rename _ => hσ
-    · intro hcon; injection hcon
-    · intro h
-      rw [litValue_fls_iff] at hσ
-      simp [hσ]
-      exact ih h
-    · rename ILit => mapped_lit
-      rw [litValue_lit_iff] at hσ
-      simp [hσ]
-      split <;> rename _ => h_mapped_lit <;> try simp
-      · intro hcon; injection hcon
-      · intro h
-        rcases ih h with ⟨ih₁, ih₂⟩
-        constructor
-        · apply le_trans _ ih₁
-          apply inf_le_inf_left
-          exact inf_le_right
-        · exact ih₂
-      · intro h
-        rcases ih h with ⟨ih₁, ih₂⟩
-        rw [← litValue?_negate_none_iff] at h_mapped_lit
-        simp [toPropFun_setLit_of_none h_mapped_lit, inf_assoc] at ih₁
-        exact ⟨ih₁, extended_trans (extended_setLitFor_of_none h_mapped_lit 0) ih₂⟩
-
-theorem assumeRATClause_error {C : IClause} {σ : PS} {τ τ' : PPA} :
-    assumeRATClause C σ τ = error τ' →
-      τ.toPropFun ≤ (PropFun.substL C σ.toSubst) ∧ extended τ τ' 0 := by
-  have ⟨C⟩ := C
-  rw [assumeRATClause, Array.foldlM_eq_foldlM_data]
-  induction' C with l ls ih generalizing τ
-  · simp [pure, Except.pure]
-  · simp; split <;> rename _ => hσ
-    · intro h; injection h; rename _ => h; subst h
-      rw [litValue_tr_iff] at hσ
-      simp [hσ]
-    · intro h
-      rw [litValue_fls_iff] at hσ
-      simp [hσ]
-      exact ih h
-    · rename ILit => mapped_lit
-      rw [litValue_lit_iff] at hσ
-      simp [hσ]
-      split <;> rename _ => h_mapped_lit <;> try simp
-      · intro h; injection h; rename _ => h; subst h
-        rw [litValue?_true_iff] at h_mapped_lit
-        exact ⟨le_trans h_mapped_lit le_sup_left, extended_refl _ _⟩
-      · intro h
-        rw [litValue?_false_iff] at h_mapped_lit
-        rcases ih h with ⟨ih₁, ih₂⟩
-        exact ⟨le_trans ih₁ le_sup_right, ih₂⟩
-      · intro h
-        rw [← litValue?_negate_none_iff] at h_mapped_lit
-        rcases ih h with ⟨ih₁, ih₂⟩
-        simp [toPropFun_setLit_of_none h_mapped_lit] at ih₁
-        constructor
-        · exact sdiff_le_iff.mp ih₁
-        · exact extended_trans (extended_setLitFor_of_none h_mapped_lit 0) ih₂
-
--- Check each clause in the formula.
--- C is the current clause in the formula to be checked for the RAT property under σ and τ
--- If C is reduced by σ, then it is RAT. Find a RAT hint and uses the RAT UP hints to derive contradiction.
---def checkClause (F : ICnf) (σ : PS) (ratHints : Array (Nat × Array Nat))
---    (p : PPA × Nat) (index : Fin F.size) (C : IClause) : Except Unit (PPA × Nat)
-
-theorem checkClause_ok {F : ICnf} {σ : PS} {ratHints : Array (Nat × Array Nat)}
-    {τ τ' : PPA} {ratIndex ratIndex' index index' bc bc' : Nat} {C : IClause} :
-    C ∈ F → uniform τ ((ratHints.size + 1) - bc) →
-      checkClause F σ ratHints ⟨τ, ratIndex, index, bc⟩ C = ok (τ', ratIndex', index', bc') →
-      F.toPropFun ⊓ τ ≤ PropFun.substL C σ.toSubst ∧
-      ((bc' = bc ∧ τ' = τ) ∨
-       (bc' = bc + 1 ∧ uniform τ' ((ratHints.size + 1) - bc') ∧ τ'.toPropFun = τ.toPropFun)) := by
-  intro hC h_uni
-  simp [checkClause]
-  split <;> rename _ => h_red
-  · simp; rintro rfl rfl rfl rfl
-    rw [reduce_satisfied_iff] at h_red
-    rw [h_red]
-    exact ⟨le_top, Or.inl ⟨rfl, rfl⟩⟩
-  · simp; rintro rfl rfl rfl rfl
-    rw [reduce_notReduced_iff] at h_red
-    rw [h_red]
-    exact ⟨inf_le_of_left_le (Cnf.le_of_mem hC), Or.inl ⟨rfl, rfl⟩⟩
-  · split <;> rename _ => hbc <;> try simp
-    split <;> rename _ => h_hint <;> try simp
-    rename Fin _ => hint_index
-    have h_bc_lt : 1 < (ratHints.size + 1) - bc := by
-      apply Nat.lt_sub_of_add_lt
-      rw [add_comm]
-      exact Nat.add_lt_add_right hbc 1
-    split <;> rename PPA => τ₂ <;> rename _ => h_RAT_assumption <;> try simp
-    · rintro rfl rfl rfl rfl
-      use inf_le_of_right_le (assumeRATClause_error h_RAT_assumption).1
-      right; use rfl
-      rcases assumeRATClause_error h_RAT_assumption with ⟨_, h₂⟩
-      exact uniform_bump_of_uniform_of_extended h_bc_lt h_uni h₂
-    · split <;> rename PPA => τ₃ <;> rename _ => h_ratHints <;> try simp
-      rintro rfl rfl rfl rfl
-      rcases assumeRATClause_ok h_RAT_assumption with ⟨h_RAT₁, h_RAT₂⟩
-      rcases fold_UP_checked h_ratHints with ⟨h₁, h₂⟩
-      have h_ext := extended_trans h_RAT₂ h₂
-      constructor
-      -- TODO: Standard form can probably remove the need for these operations
-      · rw [inf_compl_le_iff_le_sup, sup_comm, ← inf_compl_le_iff_le_sup, inf_comm] at h_RAT₁
-        rw [← le_compl_iff_inf_le_bot] at h₁
-        exact le_trans (inf_le_inf_right (PPA.toPropFun τ) h₁) h_RAT₁
-      · exact Or.inr ⟨rfl, uniform_bump_of_uniform_of_extended h_bc_lt h_uni h_ext⟩
-
-theorem fold_checkClause_ok {F F' : ICnf} {σ : PS} {ratHints : Array (Nat × Array Nat)}
-    {τ τ' : PPA} {ratIndex ratIndex' index index' bc bc' : Nat} :
-    -- TODO: Additional assumptions on τ, related to C or isSetFor
-    (∀ C ∈ F, C ∈ F') →
-    uniform τ ((ratHints.size + 1) - bc) →
-    F.foldlM (checkClause F' σ ratHints) (τ, ratIndex, index, bc) = ok (τ', ratIndex', index', bc') →
-      F'.toPropFun ⊓ τ ≤ (PropFun.substL F σ.toSubst) := by
-  intro hF h_ext
-  have ⟨F⟩ := F
-  rw [Array.foldlM_eq_foldlM_data]
-  induction' F with C CS ih generalizing τ ratIndex index bc <;> simp
-  match h_check : checkClause F' σ ratHints (τ, ratIndex, index, bc) C with
-  | error _ => intro hcon; injection hcon
-  | ok (τ₂, rI₂, i₂, bc₂) =>
-    simp [← Array.mem_data] at hF
-    rcases hF with ⟨hF₁, hF₂⟩
-    rw [Array.mem_data] at hF₁
-    simp [Array.mem_data] at hF₂
-    have : ∀ C ∈ ({ data := CS } : ICnf), C ∈ F' := by
-      simp [← Array.mem_data]; simp_rw [Array.mem_data]; exact hF₂
-    rcases checkClause_ok hF₁ h_ext h_check with ⟨h₁, h₂⟩
-    rcases h₂ with (⟨rfl, rfl⟩ | ⟨rfl, hτ₂_ext, hτ₂_propfun⟩)
-    · exact fun h => ⟨h₁, ih h_ext this h⟩
-    · intro h
-      use h₁
-      rw [← hτ₂_propfun]
-      exact ih hτ₂_ext this h
-
--- For the line to continue checking, the clause to be added must be redundant
-theorem checkLine_ok {F : ICnf} {τ : PPA} {σ : PS} {line : SRLine} {S : SRState} :
-    checkLine ⟨F, τ, σ⟩ line = ok S → eqsat F.toPropFun (F.toPropFun ⊓ line.1) := by
-  simp [checkLine]
-  rcases line with ⟨C, w_tf, w_maps, UPhints, RAThints⟩
-  split <;> try simp
-  rename PPA => τ₁
-  rename _ = ok τ₁ => h_assumeNegatedCandidate
-  rcases assumeNegatedClauseFor_ok h_assumeNegatedCandidate with ⟨hC₁, hC₂⟩
-  replace hC₂ := uniform_of_extended_reset hC₂
-  simp at hC₁ hC₂
-  --replace hC₂ := uniform_of_extended_reset hC₂
-  match h_hints : UPhints.foldlM (applyUPHint F (RAThints.size + 1)) τ₁ with
-  | error (_, .checkError) => simp
-  | error (τ', .checked) =>
-    simp; split <;> simp
-    rcases fold_UP_checked h_hints with ⟨h₁, h₂⟩
-    rw [hC₁] at h₁
-    rw [← le_iff_inf_compl_le_bot] at h₁
-    exact fun _ => eqsat_of_entails h₁
-  | ok τ₂ =>
-    simp; split <;> try simp
-    split <;> try simp
-    rename 0 < _ ∧ 0 < _ => h_sizes
-    rcases h_sizes with ⟨hC_size, hw_size⟩
-    match h_RAT : F.foldlM (checkClause F (assumeWitness σ C[0] w_tf w_maps) RAThints) (τ₂, 0, 0, 0) with
-    | error () => simp
-    | ok (τ₃, idx₃) =>
-      split <;> try simp
-      rename _ => h_ok; simp at h_ok; rcases h_ok with ⟨rfl, rfl⟩
-      rcases fold_UP_ok h_hints with ⟨h₁, h₂⟩
-      rw [hC₁] at h₁
-      intro
-      apply SR_core (assumeWitness_subst hC_size σ w_tf w_maps)
-      replace hC₂ : uniform τ₂ ((RAThints.size + 1) - 0) := uniform_of_uniform_of_extended hC₂ h₂
-      have hFC_le_Fτ₂ : F.toPropFun ⊓ (C.toPropFun)ᶜ ≤ F.toPropFun ⊓ τ₂ := by
-        have := inf_le_inf_left F.toPropFun h₁
-        rwa [← inf_assoc, inf_idem] at this
-      exact le_trans hFC_le_Fτ₂ (fold_checkClause_ok (by simp) hC₂ h_RAT)
+        match loop 0 0 0 τ with
+        | ⟨_, false⟩ => error false
+        | ⟨τ, true⟩ => ok ⟨F.commit, τ, σ⟩
+      else error false -/
 
 end SR
