Experiments/ProofChecking/SRCheckerExe.lean
@@ -1,0 +1,100 @@
+/-
+
+A runner for `SRChecker.lean`.
+
+Command-line tool for checking LSR files.
+
+Author: Cayden Codel
+Carnegie Mellon University
+
+-/
+
+import Experiments.ProofChecking.SRParser
+import Experiments.ProofChecking.SRChecker
+import Experiments.ProofChecking.RangeArray
+
+import LeanSAT.Data.Cnf
+import LeanSAT.Data.ICnf
+import LeanSAT.Data.Literal
+
+open LeanSAT LeanSAT.Model
+
+def printUsage : IO Unit := do
+  IO.println "Usage: ./SRChecker <cnf> <lsr> [c]"
+  IO.println ""
+  IO.println "where"
+  IO.println ""
+  IO.println "   [c] is an optional argument specifying that <lsr> is in binary compressed format."
+  IO.println ""
+  IO.println "If no command-line arguments are given, prints this help message."
+  IO.println "Reads the CNF and LSR files and checks the LSR proof."
+
+def interpretResult : Except Bool SRState → IO Unit
+  | .ok _ => do
+    IO.println "c Proof is valid, but did not derive the empty clause."
+    IO.println "s VALID"
+  | .error true => do
+    IO.println "c Proof derived the empty clause"
+    IO.println "s VERIFIED UNSAT"
+  | .error false => do
+    IO.println "c Error or invalid proof"
+    IO.println "s INVALID"
+
+partial def main : List String → IO Unit
+  | [] => printUsage
+  | [_] => printUsage
+  | [cnfFile, lsrFile] => do
+    let cnfContents ← IO.FS.withFile cnfFile .read (·.readToEnd)
+    let (F, nvars) ← IO.ofExcept <| SRParser.parseFormula cnfContents (RangeArray.empty : RangeArray ILit)
+
+    let lsrContents ← IO.FS.withFile lsrFile .read (·.readToEnd)
+    let lines := lsrContents.splitOn "\n"
+    interpretResult <| lines.foldlM (init := SR.SRState.mk F (PPA.new (nvars * 2)) (PS.new (nvars * 2))) (fun st line =>
+      match SRParser.parseLSRLine st.F line with
+      | .error str =>
+        dbg_trace s!"Error: {str}"
+        .error false
+      | .ok (id, F, pl) =>
+        let st := { st with F := F.commitUntil (id - 1) }
+        match pl with
+        | .inl addLine =>
+          SR.checkLine st addLine
+        | .inr delLine =>
+          delLine.clauses.foldlM (fun st clauseId =>
+            if hc : clauseId < st.F.size then
+              if st.F.isDeletedFin ⟨clauseId, hc⟩ then
+                .error false
+              else
+                .ok { st with F := st.F.deleteFin ⟨clauseId, hc⟩ }
+            else .error false) st)
+  | [cnfFile, lsrFile, "c"] => do
+    let cnfContents ← IO.FS.withFile cnfFile .read (·.readToEnd)
+    let (F, nvars) ← IO.ofExcept <| SRParser.parseFormula cnfContents (RangeArray.empty : RangeArray ILit)
+
+    let bytes ← IO.FS.withFile lsrFile .read (·.readBinToEnd)
+    let b_size := bytes.size
+    let rec loop (index : Nat) (st : SR.SRState) : Except Bool SR.SRState :=
+      if index < b_size then
+        match SRParser.parseLSRLineBinary st.F bytes index with
+        | .error str =>
+          dbg_trace s!"Error: {str}"
+          .error false
+        | .ok (index, id, F, pl) =>
+          let st := { st with F := F.commitUntil (id - 1) }
+          match pl with
+          | .inl addLine =>
+            match SR.checkLine st addLine with
+            | .ok st => loop index st
+            | .error b => .error b
+          | .inr delLine =>
+            delLine.clauses.foldlM (fun st clauseId =>
+              if hc : clauseId < st.F.size then
+                if st.F.isDeletedFin ⟨clauseId, hc⟩ then
+                  .error false
+                else
+                  .ok { st with F := st.F.deleteFin ⟨clauseId, hc⟩ }
+              else .error false) st
+      else .error false
+    interpretResult <| loop 0 (SR.SRState.mk F (PPA.new (nvars * 2)) (PS.new (nvars * 2)))
+
+  | _ => printUsage
