Experiments/ProofChecking/SRParser.lean
@@ -1,276 +1,460 @@
 /-
 
-A parser for the LSR proof format.
+An SR parser (and updated CNF formula parser).
+Made general via a `SRParser.Formula` class.
 
-Authors: Cayden Codel
+Author: Cayden Codel
 Carnegie Mellon University
 
 -/
 
 import LeanSAT.Solver.Dimacs
 import Experiments.ProofChecking.RangeArray
-import Experiments.ProofChecking.SRChecker
-
-import Std
 
 open Std
 open LeanSAT.Solver.Dimacs
-open LeanSAT LeanSAT.Model ILit
+open LeanSAT LeanSAT.Model ILit Except
+
+namespace SR
+
+structure SRAdditionLine where
+  witnessLits : Array ILit     -- Maps literals to true/false
+  witnessMaps : Array ILit     -- Maps variables to literals
+  upHints : Array Nat          -- Already 0-indexed clause IDs into the accumulated formula
+  ratHintIndexes : Array Nat   -- Already 0-indexed
+  ratHints : Array (Array Nat) -- Already 0-indexed
+  ratSizesEq : ratHintIndexes.size = ratHints.size
+  witnessMapsMod : witnessMaps.size % 2 = 0
+  -- CC: Technically, ratHints can be a RangeArray. Try later
+
+def SRAdditionLine.new : SRAdditionLine := ⟨
+  Array.mkEmpty 100,
+  Array.mkEmpty 100,
+  Array.mkEmpty 100,
+  Array.mkEmpty 100,
+  Array.mkEmpty 100,
+  by simp, by simp⟩
+
+instance : Inhabited SRAdditionLine := ⟨{
+  witnessLits := #[],
+  witnessMaps := #[],
+  upHints := #[],
+  ratHintIndexes := #[],
+  ratHints := #[],
+  ratSizesEq := by simp,
+  witnessMapsMod := by simp
+}⟩
+
+structure SRDeletionLine where
+  clauses : Array Nat
+deriving Inhabited
+
+end SR
 
 namespace SRParser
 
-open Except
-open SR
-
-universe u
-
-/-- The type `L` is a representation of literals over variables of type `ν`. -/
-class Formula (F : Type u) where
+protected class Formula (F : Type _) where
   empty : F
-  addClause : F → IClause → F
+  addLiteral : F → ILit → F
+  commitClause : F → F
   size : F → Nat
 
-instance : Formula (RangeArray ILit) where
+instance : SRParser.Formula (RangeArray ILit) where
   empty := (RangeArray.empty : RangeArray ILit)
-  addClause := RangeArray.add
+  addLiteral := RangeArray.push
+  commitClause := RangeArray.commit
   size := RangeArray.size
 
-instance : Formula (ICnf) where
-  empty := #[]
-  addClause := (fun F C => Cnf.addClause C F)
-  size := Array.size
+instance : SRParser.Formula (ICnf × IClause) where
+  empty := (#[], #[])
+  addLiteral := (fun ⟨F, C⟩ l => ⟨F, C.push l⟩)
+  commitClause := (fun ⟨F, C⟩ => (F.push C, #[]))
+  size := (fun ⟨F, _⟩ => F.size)
 
-structure ArrayParseRes where
-  vars : Nat
-  clauses : ICnf
+variable {CNF : Type _} [SRParser.Formula CNF]
 
-structure RAPraseRes where
-  vars : Nat
-  formula : RangeArray ILit
-
-def parseLit (maxVar : Nat) (C : IClause) (s : String) : Except (Except String IClause) IClause := do
+-- Parses a single literal from a string.
+-- CC: The double Except monad is used to stop folding across a list/array of atom strings
+--     in case a 0 is encountered, since DIMACS doesn't require a clause to fit on a line.
+@[inline, specialize]
+def parseLitM (maxVar : Nat) (F : CNF) (s : String) : Except (Except String CNF) CNF := do
   match s.toInt? with
   | none => throw (throw s!"Literal is not a number: {s}")
   | some n =>
     if hn : n = 0 then
-      throw (return C)
+      throw (return F)
     else
       if n.natAbs > maxVar then
         throw (throw s!"Literal {n} is greater than the maximum variable {maxVar}")
       else
-        if n < 0 then
-          return C.push ⟨n, hn⟩
-        else
-          return C.push ⟨n, hn⟩
+        return Formula.addLiteral F ⟨n, hn⟩
 
-def parseClause {α : Type} [Formula α] (maxVar : Nat) (F : α) (s : String) : Except String α :=
-  match s.splitOn " " |>.foldlM (parseLit maxVar) #[] with
-  | ok _ => throw "Zero not encountered on this line"
-  | error e => return Formula.addClause F (← e)
+inductive DimacsParsingResult
+  | ok         -- Parsing expects more input
+  | done       -- Parsing expects to be done
+  | err : String → DimacsParsingResult   -- Error encountered
+  deriving Inhabited, DecidableEq
 
--- Parses the CNF given a string and an empty formula to read the clauses into
-def parseFormula {α : Type} [Formula α] (s : String) (F : α) : Except String α := do
-  let ⟨pLine, clauseLines⟩ ←
-    s.splitOn "\n"
-    |>.filter (fun line => !line.startsWith "c" && line.any (!·.isWhitespace))
-    |>.expectNonempty fun () => "All lines are empty or comments"
-  let (nvars, ncls) ← parseHeader pLine
-  let F ← clauseLines.foldlM (parseClause nvars) F
-  if Formula.size F != ncls then
-    throw s!"Expected {ncls} clauses, but found {Formula.size F}"
-  else
-    return F
-
-inductive LPRCheckingMode
-| Clause   : LPRCheckingMode
-| Witness  : LPRCheckingMode
-| Reducing : LPRCheckingMode
-| DoneWithLine : LPRCheckingMode
-deriving BEq
-
-inductive SRParsingMode
-| clause
-| witness_tf
-| witness_mapped_ready
-| witness_mapped_halfway : IVar → SRParsingMode
-| up_hints
-| rat_hints : Nat × Array Nat → SRParsingMode
-| done_with_line -- Could be removed, in favor of Except (Except String SRLine), but this is arguably more elegant
-deriving BEq
-
-open SRParsingMode
-
-structure SRDeletionLine where
-  clauses : Array Nat
-
-def parseSRAtom (pivot : Option ILit) (p : SRLine × SRParsingMode) (s : String) : Except String (SRLine × SRParsingMode) :=
-  let ⟨line, mode⟩ := p
-  -- No matter what, the string should be a number, so parse it as an int
+-- Parses a single literal from a string. Keeps track of whether a '0' has been found.
+@[inline, specialize]
+def parseLit (maxVar : Nat) (F : CNF) (s : String) : DimacsParsingResult × CNF :=
   match s.toInt? with
-  | none => throw s!"Atom {s} didn't parse to a number"
+  | none => (.err s!"Literal '{s}' is not a number.", F)
   | some n =>
     if hn : n = 0 then
-      match mode with
-      | .clause =>
-        -- We don't have a witness, so we insert the pivot into the witness and continue, if the clause isn't empty
-        match pivot with
-        | none => return ⟨line, .up_hints⟩
-        | some pivot => return ⟨{ line with witness_lits := line.witness_lits.push pivot }, .up_hints⟩
-      | .witness_tf => return ⟨line, .up_hints⟩
-      | .witness_mapped_ready => return ⟨line, .up_hints⟩
-      | .witness_mapped_halfway _ => throw s!"Only got half a substitution mapping when ending a witness"
-      | .up_hints => return ⟨line, .done_with_line⟩
-      | .rat_hints hints => return ⟨{ line with rat_hints := line.rat_hints.push hints }, .done_with_line⟩
-      | .done_with_line => throw s!"Addition line continued after last ending 0"
+      (.done, F)
     else
-      match mode with
-      | .clause =>
-        match pivot with
-        | none => throw "No pivot provided for the clause"
-        | some pivot =>
-          if n = pivot.val then
-            -- Seeing the pivot again means we're parsing a witness
-            return ⟨{ line with witness_lits := line.witness_lits.push ⟨n, hn⟩ }, .witness_tf⟩
-          else
-            -- It's not the pivot (and it's not 0), so add it to the clause
-            return ⟨{ line with clause := line.clause.push ⟨n, hn⟩ }, .clause⟩
-      | .witness_tf =>
-        match pivot with
-        | none => throw "No pivot provided for the witness"
-        | some pivot =>
-          if n = pivot.val then
-            -- Seeing the pivot again means we're parsing the substitution mappings
-            return ⟨line, .witness_mapped_ready⟩
-          else
-            return ⟨{ line with witness_lits := line.witness_lits.push ⟨n, hn⟩ }, .witness_tf⟩
-      | .witness_mapped_ready =>
-        match pivot with
-        | none => throw "No pivot provided for the witness"
-        | some pivot =>
-          if n = pivot.val then
-            throw s!"Saw pivot again in substitution mapping"
-          else
-            if n < 0 then
-              throw s!"First of a substitution mapping must be positive"
-            else
-              return ⟨line, .witness_mapped_halfway ⟨n.natAbs, Int.natAbs_pos.mpr hn⟩⟩
-      | .witness_mapped_halfway v =>
-        return ⟨{line with witness_maps := line.witness_maps.push ⟨v, ⟨n, hn⟩⟩ }, .witness_mapped_ready⟩
-      | .up_hints =>
-        if n < 0 then
-          match pivot with
-          | none => throw "Can't have RAT hints for empty clauses"
-          | _ =>
-            -- This is our first RAT hint - start building it
-            return ⟨line, .rat_hints ⟨n.natAbs - 1, #[]⟩⟩
-        else
-          return ⟨{ line with up_hints := line.up_hints.push (n.natAbs - 1) }, .up_hints⟩
-      | .rat_hints ⟨h, hints⟩ =>
-        if n < 0 then
-          -- This is a new RAT hint - add the old one
-          return ⟨{ line with rat_hints := line.rat_hints.push ⟨h, hints⟩ }, .rat_hints ⟨n.natAbs - 1, #[]⟩⟩
-        else
-          return ⟨line, .rat_hints ⟨h, hints.push (n.natAbs - 1)⟩⟩
-      | .done_with_line => throw s!"Addition line continued after last ending 0"
+      if n.natAbs > maxVar then
+        (.err s!"Literal {n} is greater than the maximum variable {maxVar}.", F)
+      else
+        (.ok, Formula.addLiteral F ⟨n, hn⟩)
 
-def parseLSRLine (p : Nat × Array (SRLine ⊕ SRDeletionLine)) (s : String) : Except String (Nat × Array (SRLine ⊕ SRDeletionLine)) :=
-  let ⟨maxId, lines⟩ := p
+@[specialize]
+def parseClauseM (maxVar : Nat) (F : CNF) (s : String) : Except String CNF :=
+  match s.splitOn " " |>.foldlM (parseLitM maxVar) F with
+  | ok _ => throw "Zero not encountered on this line"
+  | error e => return Formula.commitClause (← e)
+
+@[specialize]
+def parseClause (maxVar : Nat) (F : CNF) (s : String) : DimacsParsingResult × CNF :=
+  let rec loop (F : CNF) : List String → DimacsParsingResult × CNF
+    | [] => (.err "0 not found before end of line", F)
+    | atom :: atoms =>
+      match parseLit maxVar F atom with
+      | (.err str, F) => (.err str, F)
+      | (.ok, F) => loop F atoms
+      | (.done, F) =>
+        if atoms.length = 0 then
+          (.done, Formula.commitClause F)
+        else
+          (.err "0 found before end of line", F)
+  loop F (s.splitOn " ")
+
+-- Parses the CNF given a string and an empty formula to read the clauses into
+@[specialize]
+def parseFormulaM (s : String) (F : CNF) : Except String (CNF × Nat) := do
+  match s.splitOn "\n" |>.filter (fun line => !line.startsWith "c" && line.any (!·.isWhitespace)) with
+  | [] => throw "All lines are empty or comments"
+  | (pLine :: clauseLines) =>
+    let (nvars, ncls) ← parseHeader pLine
+    let F ← clauseLines.foldlM (parseClauseM nvars) F
+    if SRParser.Formula.size F != ncls then
+      throw s!"Expected {ncls} clauses, but found {Formula.size F}"
+    else
+      return (F, nvars)
+
+-- CC: Because `parseFormula` is only called at top level once, it is okay to
+--     have the return type be an `Except` monad. However, the functions called
+--     by this function are the non-monadic versions.
+@[specialize]
+def parseFormula (s : String) (F : CNF) : Except String (CNF × Nat) :=
+  match s.splitOn "\n" |>.filter (fun line => !line.startsWith "c" && line.any (!·.isWhitespace)) with
+  | [] => throw "All lines are empty or comments"
+  | (pLine :: clauseLines) =>
+    match parseHeader pLine with
+    | .error str => throw str
+    | .ok (nvars, ncls) =>
+      let rec loop (F : CNF) : List String → Except String CNF
+        | [] =>
+          if SRParser.Formula.size F != ncls then
+            throw s!"Expected {ncls} clauses, but found {Formula.size F}"
+          else
+            ok F
+        | c :: cs =>
+          match parseClause nvars F c with
+          | (.err str, _) => throw str
+          | (_, F) => loop F cs    -- We should expect .done here, but .ok works too
+      match loop F clauseLines with
+      | .ok F => ok (F, nvars)
+      | .error str => throw str
+
+inductive SRParsingMode
+  | clause
+  | witnessLits
+  | witnessMappedReady
+  | witnessMappedHalfway : IVar → SRParsingMode
+  | upHints
+  | ratHints : Nat → Array Nat → SRParsingMode
+  | lineDone
+  | err : String → SRParsingMode
+  deriving BEq, DecidableEq, Inhabited
+
+open SR SRParsingMode
+
+structure ParsingState (CNF : Type _) where
+  mode : SRParsingMode
+  pivot : Option ILit
+  F : CNF
+  line : SRAdditionLine
+
+@[inline]
+def processSRAtom (atom : Int) (st : ParsingState CNF) : ParsingState CNF :=
+  if h_atom : atom = 0 then
+    match st.mode with
+    | .clause =>
+      -- We don't have a witness, so we insert the pivot into the witness and continue, if the clause isn't empty
+      match st.pivot with
+      | none => { st with mode := .upHints }
+      | some pivot => { st with
+        line := { st.line with witnessLits := st.line.witnessLits.push pivot },
+        mode := .upHints }
+    | .witnessLits => { st with mode := .upHints }
+    | .witnessMappedReady => { st with mode := .upHints }
+    | .witnessMappedHalfway _ => { st with mode := .err "Only got half a substitution mapping when ending a witness" }
+    | .upHints => { st with mode := .lineDone }
+    | .ratHints index hints => { st with
+        mode := .lineDone,
+        line := { st.line with
+          ratHintIndexes := st.line.ratHintIndexes.push index,
+          ratHints := st.line.ratHints.push hints,
+          ratSizesEq := by simp; exact st.line.ratSizesEq }
+        }
+    | .lineDone => { st with mode := .err "Addition line continued after last ending 0" }
+    | .err str => { st with mode := .err str }
+  else
+    match st.mode with
+    | .clause =>
+      match st.pivot with
+      | none => { st with mode := .err "No pivot provided for the clause" }
+      | some pivot =>
+        if atom = pivot.val then
+          -- Seeing the pivot again means we're parsing a witness
+          { st with
+            mode := .witnessLits,
+            line := { st.line with witnessLits := st.line.witnessLits.push pivot }
+          }
+        else
+          -- It's not the pivot (and it's not 0), so add it to the clause
+          { st with
+            F := Formula.addLiteral st.F ⟨atom, h_atom⟩,
+            mode := .clause
+          }
+    | .witnessLits =>
+      match st.pivot with
+      | none => { st with mode := .err "No pivot provided for the witness" }
+      | some pivot =>
+        if atom = pivot.val then
+          -- Seeing the pivot again means we're parsing the substitution mappings
+          { st with mode := .witnessMappedReady }
+        else
+          { st with
+            line := { st.line with witnessLits := st.line.witnessLits.push ⟨atom, h_atom⟩ },
+            mode := .witnessLits
+          }
+    | .witnessMappedReady =>
+      match st.pivot with
+      | none => { st with mode := .err "No pivot provided for the witness" }
+      | some pivot =>
+        if atom = pivot.val then
+          { st with mode := .err "Saw pivot again in substitution mapping" }
+        else
+          if atom < 0 then
+            { st with mode := .err "First of a substitution mapping must be positive" }
+          else
+            { st with mode := .witnessMappedHalfway ⟨atom.natAbs, Int.natAbs_pos.mpr h_atom⟩ }
+    | .witnessMappedHalfway v =>
+      { st with
+        mode := .witnessMappedReady,
+        line := { st.line with
+          witnessMaps := st.line.witnessMaps.push v |>.push ⟨atom, h_atom⟩,
+          witnessMapsMod := by simp [add_assoc, Nat.add_mod_right]; exact st.line.witnessMapsMod }
+       }
+    | .upHints =>
+      if atom < 0 then
+        match st.pivot with
+        | none => { st with mode := .err "Can't have RAT hints for empty clauses" }
+        | _ =>
+          -- This is our first RAT hint - start building it
+          { st with mode := .ratHints (atom.natAbs - 1) #[] }
+      else
+        { st with
+          mode := .upHints
+          line := { st.line with upHints := st.line.upHints.push (atom.natAbs - 1) }
+        }
+    | .ratHints index hints =>
+      if atom < 0 then
+        -- This is a new RAT hint - add the old one
+        { st with
+          mode := .ratHints (atom.natAbs - 1) #[],
+          line := { st.line with
+            ratHintIndexes := st.line.ratHintIndexes.push index,
+            ratHints := st.line.ratHints.push hints,
+            ratSizesEq := by simp; exact st.line.ratSizesEq }
+        }
+      else
+        { st with mode := .ratHints index (hints.push (atom.natAbs - 1)) }
+    | .lineDone =>
+      { st with mode := .err "Addition line continued after last ending 0" }
+    | .err str =>
+      { st with mode := .err str }
+
+def parseSRAtom (st : ParsingState CNF) (s : String) : ParsingState CNF :=
+  -- No matter what, the string should be a number, so parse it as an int
+  match s.toInt? with
+  | none => { st with mode := .err s!"Atom {s} didn't parse to a number" }
+  | some n => processSRAtom n st
+
+-- CC: Because the parse line is called at top-level, it's okay for this to be Except.
+-- Returns the line id, the updated formula (with the candidate clause loaded), and the line
+def parseLSRLine (F : CNF) (s : String) : Except String (Nat × CNF × (SRAdditionLine ⊕ SRDeletionLine)) :=
   match s.splitOn " " with
   | [] => throw "Empty line"
-  | [_] => throw s!"Single atom line: {s}, with id {maxId}"
+  | [id] => throw s!"Single atom line: {s}, with id {id}"
   | (id :: hd :: tls) =>
-    match hd with
-    | "d" =>
-      -- Check to make sure the maxId is (non-strictly) monotonically increasing
-      match id.toNat? with
-      | none => throw "Line ID is not a number"
-      | some id =>
-        if id < maxId then
-          throw "Deletion line id is not increasing"
-        else
-          match tls.foldlM (fun arr str =>
-            match str.toNat? with
-            | none => throw (throw s!"{str} was not a number")
-            | some 0 => throw (return arr)
-            | some (n + 1) => return arr.push n) #[] with
-          | ok _ => throw "Zero not found on deletion line"
-          | error e => return ⟨max id maxId, lines.push (.inr (SRDeletionLine.mk (← e)))⟩
-    | _ =>
+    match id.toNat? with
+    | none => throw s!"Line ID {id} is not a number"
+    | some id =>
+      match hd with
+      | "d" =>
+        -- Check to make sure the maxId is (non-strictly) monotonically increasing
+        -- CC: We actually don't care about this, since we assume the proof is ordered.
+        match tls.foldlM (fun arr str =>
+          match str.toNat? with
+          | none => throw (throw s!"{str} was not a number")
+          | some 0 => throw (return arr)
+          | some (n + 1) => return arr.push n) #[] with
+        | ok _ => throw "Zero not found on deletion line"
+        | error e => return ⟨id, F, .inr (SRDeletionLine.mk (← e))⟩
+      | _ =>
       -- We have an addition line, so the maxId should strictly increase
-      match id.toNat? with
-      | none => throw "Line ID is not a number"
-      | some id =>
-        if id ≤ maxId then
-          throw s!"Addition line id is not increasing: parsed {id}, max {maxId}"
-        else
-          match hd.toInt? with
-          | none => throw "Pivot is not a number"
-          | some n =>
-            let line : SRLine := ⟨#[], #[], #[], #[], #[]⟩
+        -- CC: Similarly, we don't care that the ID line is strictly increasing,
+        --     only that the clause doesn't exist in the formula yet.
+        match hd.toInt? with
+        | none => throw "Pivot is not a number"
+        | some n =>
+          let line := SRAdditionLine.new
+          let st :=
             if hn : n = 0 then
-              match tls.foldlM (parseSRAtom none) ⟨line, .up_hints⟩ with
-              | error str => throw str
-              | ok ⟨line, mode⟩ =>
-                if mode != .done_with_line then
-                  throw "Addition line for empty clause didn't end with 0"
-                else
-                  return ⟨id, lines.push (.inl line)⟩
+              ParsingState.mk .upHints none F line
             else
-              match tls.foldlM (parseSRAtom (some ⟨n, hn⟩)) ⟨{ line with clause := line.clause.push ⟨n, hn⟩ }, .clause⟩ with
-              | error str => throw str
-              | ok ⟨line, mode⟩ =>
-                if mode != .done_with_line then
-                  throw "Addition line didn't end with 0"
-                else
-                  return ⟨id, lines.push (.inl line)⟩
+              ParsingState.mk .clause (some ⟨n, hn⟩) (SRParser.Formula.addLiteral F ⟨n, hn⟩) line
 
-def parseLSRFile (formulaSize : Nat) (s : String) : Except String (Array (SRLine ⊕ SRDeletionLine)) :=
-  match s.splitOn "\n"
-    |>.filter (fun line => !line.startsWith "c" && line.any (!·.isWhitespace))
-    |>.foldlM parseLSRLine ⟨formulaSize, #[]⟩ with
-  | error e => throw e
-  | ok ⟨_, lines⟩ => return lines
+          let rec loop (st : ParsingState CNF) : List String → ParsingState CNF
+            | [] => st
+            | atom :: atoms =>
+              let st := parseSRAtom st atom
+              match st.mode with
+              | .err _ => st
+              | _ => loop st atoms
 
+          let st := loop st tls
+          match st.mode with
+          | .err str => throw str
+          | .lineDone => return ⟨id, st.F, .inl st.line⟩
+          | _ => throw "Addition line didn't end with 0"
+
+--------------------------------------------------------------------------------
+
+def undoBinaryMapping (x : UInt64) : Int :=
+  if x &&& 1 = 1 then
+    ((((x >>> 1).toNat) : Int) * -1)
+  else
+    (((x >>> 1).toNat) : Int)
+
+-- CC: This version is an attempt to get totality
+/-
+def readBinaryToken (A : ByteArray) (index : Nat) : Int × { i : Nat // i > index } :=
+  let rec go (i : Nat) (acc : UInt64) (shift : UInt64) : Int × { idx : Nat // idx > i } :=
+    if hi : i < A.size then
+      let atom : UInt8 := A.get ⟨i, hi⟩
+      let acc' : UInt64 := acc ||| ((atom &&& 127).toUInt64 <<< shift)
+      if atom &&& 128 != 0 then
+        match go (i + 1) acc' (shift + 7) with
+        | ⟨a, ⟨b, hb⟩⟩ => ⟨a, ⟨b, Nat.le_of_succ_le hb⟩⟩
+      else
+        ⟨undoBinaryMapping acc', ⟨A.size, hi⟩⟩
+    else
+      ⟨undoBinaryMapping acc, ⟨i + 1, Nat.lt_succ_self _⟩⟩
+  termination_by A.size - i
+  go index 0 0
+-/
+
+-- Int is result, Nat is cached index into A
+partial def readBinaryToken (A : ByteArray) (index : Nat) : Int × Nat :=
+  let rec go (i : Nat) (acc : UInt64) (shift : UInt64) : Int × Nat :=
+    if hi : i < A.size then
+      let atom : UInt8 := A.get ⟨i, hi⟩
+      let acc' : UInt64 := acc ||| ((atom &&& 127).toUInt64 <<< shift)
+      if atom &&& 128 != 0 then
+        go (i + 1) acc' (shift + 7)
+      else
+        ⟨undoBinaryMapping acc', i + 1⟩
+    else
+      ⟨undoBinaryMapping acc, A.size⟩
+  let ⟨res, idx⟩ := go index 0 0
+  -- dbg_trace s!"Pointer at index {index} moved to {idx}, parsed {res}"
+  ⟨res, idx⟩
+
+-- Bool: found a 0
+-- Nat: updated index
+partial def parseLSRDeletionLineBinary (A : ByteArray) (index : Nat) : Bool × Nat × SRDeletionLine :=
+  let rec go (i : Nat) (acc : Array Nat) : Bool × Nat × SRDeletionLine :=
+    if i < A.size then
+      let (x, j) := readBinaryToken A i
+      if x = 0 then
+        ⟨true, j, SRDeletionLine.mk acc⟩
+      else
+        go j (acc.push (x.natAbs - 1))
+    else
+      ⟨false, A.size, SRDeletionLine.mk acc⟩
+  go index #[]
+
+instance : Inhabited (Nat × ParsingState CNF) :=
+  ⟨⟨0, ParsingState.mk .clause none (SRParser.Formula.empty) (SRAdditionLine.new)⟩⟩
+
+@[specialize]
+partial def parseLSRAdditionLineBinary (F : CNF) (A : ByteArray)
+    (index : Nat) (pivot : Option ILit) : Nat × ParsingState CNF :=
+  let rec go (i : Nat) (st : ParsingState CNF) : Nat × ParsingState CNF :=
+    have : Inhabited (Nat × ParsingState CNF) := by infer_instance
+    if i < A.size then
+      let (n, j) := readBinaryToken A i
+      let st := processSRAtom n st
+      match st.mode with
+      | .err _ => (j, st)
+      | .lineDone => (j, st)
+      | _ => go j st
+    else
+      ⟨A.size, st⟩
+
+  let newLine := SRAdditionLine.new
+  match pivot with
+  | none => go index (ParsingState.mk .upHints none F newLine)
+  | some p => go index (ParsingState.mk .clause (some p) (SRParser.Formula.addLiteral F p) newLine)
+
+-- First nat is cached index into arr, second is ID of new clause to add
+partial def parseLSRLineBinary (F : CNF) (A : ByteArray) (index : Nat)
+    : Except String (Nat × Nat × CNF × (SRAdditionLine ⊕ SRDeletionLine)) :=
+  if hi : index + 1 < A.size then
+    -- Check if we have an addition line or a deletion line
+    let lineStart : UInt8 := A.get ⟨index, Nat.lt_of_succ_lt hi⟩
+    let ⟨lineId, index⟩ := readBinaryToken A (index + 1)
+    if lineId < 0 then error "Negative line ID" else
+
+    -- Addition line
+    if lineStart = 1 then
+      -- Check if we have a pivot
+      if index < A.size then
+        let ⟨pivot, index⟩ := readBinaryToken A index
+        let ⟨index, st⟩ :=
+          if hp : pivot = 0 then
+            parseLSRAdditionLineBinary F A index none
+          else
+            parseLSRAdditionLineBinary F A index (some ⟨pivot, hp⟩)
+        match st.mode with
+        | .err str => throw str
+        | .lineDone => ok (index, lineId.natAbs, st.F, .inl st.line)
+        | _ => error "Addition line didn't end with 0"
+      else
+        error "Line ended early"
+    else if lineStart = 2 then
+      match parseLSRDeletionLineBinary A index with
+      | ⟨true, index, line⟩ => ok (index, lineId.natAbs, F, .inr line)
+      | ⟨false, _, _⟩ => error "Deletion line didn't end with 0"
+    else
+      error "Start of line wasn't addition (1) or deletion (2)"
+
+  else
+    error "No more string!"
 
 end SRParser
-
-def main (args : List String) : IO Unit := do
-  let cnfFile := args[0]!
-  let lsrFile := args[1]!
-  let contents ← IO.FS.withFile cnfFile .read (·.readToEnd)
-  --let res ← fromFileEnc cnfFile
-  let F ← IO.ofExcept <| SRParser.parseFormula contents RangeArray.empty
-  --let cnf ← IO.ofExcept <| SRParser.parseFormula contents (#[] : ICnf)
-  IO.println s!"Formula has {F.size} clauses"
-  --IO.println s!"Formula has {cnf.size} clauses"
-
-  let lsrContents ← IO.FS.withFile lsrFile .read (·.readToEnd)
-  let lines ← IO.ofExcept <| SRParser.parseLSRFile (F.size) lsrContents
-  --IO.println s!"LSR file has {lines.size} lines"
-  --IO.println s!"{F}"
-  --for line in lines do
-  --  match line with
-  --  | .inl l => IO.println s!"{l.clause} {l.witness_lits} p {l.witness_maps} 0 {l.up_hints} {l.rat_hints} 0"
-  --  | .inr _ => continue
-
-  match lines.foldlM (init := ⟨F, PPA.new 100, PS.new 100⟩)
-    (fun S line =>
-      match line with
-      | .inl l => SR.checkLineFlat S l
-      | .inr l =>
-        let ⟨F, τ, σ⟩ := S
-        return ⟨l.clauses.foldl RangeArray.delete F, τ, σ⟩) with
-  | Except.ok _ => IO.println "c Flat Proof failed to derive the empty clause, but is otherwise valid"
-  | Except.error false => IO.println "c Flat Proof failed"
-  | Except.error true => IO.println "s VERIFIED UNSAT"
-
-
-  /-
-  match lines.foldlM (init := (⟨cnf, PPA.new 100, PS.new 100⟩ : SR.SRState)) ((fun S line =>
-    match line with
-    | .inl l => SR.checkLine S l
-    | .inr _ => throw false)) with
-  | .ok _ => IO.println s!"Proof was valid but failed to derive the empty clause"
-  | .error true => IO.println "s VERIFIED UNSAT"
-  | .error false => IO.println "c Proof failed"
--/
