Experiments/ProofChecking/SRParserExe.lean
@@ -1,0 +1,125 @@
+/-
+
+An executable for `SRParser.lean`.
+
+A simple command-line tool for reading in CNF/LSR files.
+What's read is echoed back to `stdout`.
+
+Author: Cayden Codel
+Carnegie Mellon University
+
+-/
+
+import Experiments.ProofChecking.SRParser
+import Experiments.ProofChecking.RangeArray
+
+import LeanSAT.Data.Cnf
+import LeanSAT.Data.ICnf
+import LeanSAT.Data.Literal
+
+open LeanSAT LeanSAT.Model
+
+def printUsage : IO Unit := do
+  IO.println "Usage: ./SRParserExe <file-path> [cnf | lsr | clsr]"
+  IO.println ""
+  IO.println "where"
+  IO.println ""
+  IO.println "  cnf: parses a CNF file."
+  IO.println "  lsr: parses an LSR file (default behavior)."
+  IO.println "  clsr: parses a compressed binary LSR file."
+  IO.println ""
+  IO.println "If no command-line arguments are given, prints this help message."
+  IO.println "Parses the CNF/LSR file and echoes it to stdout."
+  IO.println "Note that the output will be in text format, even if the input is binary."
+
+def echoCnf (filePath : String) : IO Unit := do
+  let contents ← IO.FS.withFile filePath .read (·.readToEnd)
+  match SRParser.parseFormula contents (RangeArray.empty : RangeArray ILit) with
+  | .error str => IO.println str
+  | .ok (F, nvars) =>
+    IO.println s!"p cnf {nvars} {F.size}"
+    let rec loop (i : Nat) : IO Unit := do
+      if i < F.size then
+        IO.print <| F.foldl_index (fun str lit => str ++ s!"{lit} ") "" i
+        IO.println "0"
+        loop (i + 1)
+    termination_by F.size - i
+    loop 0
+
+@[specialize]
+def echoLSRLine (F : RangeArray ILit) (id : Nat) (line : SR.SRAdditionLine) : IO Unit := do
+  let usize := F.usize
+  let F := F.commit
+
+  -- Print the line back
+  if usize > 0 then
+    IO.print <| F.foldl_index (fun str lit => str ++ s!"{lit} ") "" (F.size - 1)
+
+  if line.witnessLits.size > 1 ∨ line.witnessMaps.size > 0 then
+    --IO.print s!"WEVE DETERMINED THAT {line.witnessLits.size} and {line.witnessMaps.size} "
+    IO.print <| line.witnessLits.foldl (fun str lit => str ++ s!"{lit} ") ""
+
+    if line.witnessMaps.size > 0 then
+      IO.print s!"{line.witnessLits[0]!} "
+      IO.print <| line.witnessMaps.foldl (fun str lit => str ++ s!"{lit} ") ""
+
+  IO.print "0 "
+
+  if line.upHints.size > 0 then
+    IO.print <| line.upHints.foldl (fun str hint => str ++ s!"{hint + 1} ") ""
+
+  if line.ratHintIndexes.size > 0 then
+    IO.print <| Fin.foldl line.ratHintIndexes.size (init := "") (fun str idx =>
+      let str := str ++ s!"-{line.ratHintIndexes.get idx + 1} "
+      (line.ratHints.get ⟨idx.val, by
+        rcases idx with ⟨idx, hlt⟩
+        rwa [line.ratSizesEq] at hlt⟩).foldl (fun str hint =>
+        str ++ s!"{hint + 1} ") str)
+  IO.println "0"
+
+def echoLSR (filePath : String) : IO Unit := do
+  let contents ← IO.FS.withFile filePath .read (·.readToEnd)
+  let lines := contents.splitOn "\n"
+  lines.foldlM (fun _ line => do
+    -- Skip empty lines
+    if line.length > 0 then
+      match SRParser.parseLSRLine (RangeArray.empty : RangeArray ILit) line with
+      | .error str =>
+        IO.println s!"Error encountered: {str}"
+      | .ok ⟨id, F, pl⟩ =>
+        IO.print s!"{id} "
+        match pl with
+        | .inl addLine => echoLSRLine F id addLine
+        | .inr delLine =>
+          IO.print "d "
+          IO.print <| delLine.clauses.foldl (fun str clause => str ++ s!"{clause + 1} ") ""
+          IO.println "0") ()
+
+partial def echoLSRBinary (filePath : String) : IO Unit := do
+  let contents ← IO.FS.withFile filePath .read (·.readBinToEnd)
+  let rec loop (index : Nat) : IO Unit :=
+    if index < contents.size then
+      match SRParser.parseLSRLineBinary (RangeArray.empty : RangeArray ILit) contents index with
+      | .error str => IO.println str
+      | .ok (index, id, F, pl) => do
+        IO.print s!"{id} "
+        match pl with
+        | .inl addLine => echoLSRLine F id addLine
+        | .inr delLine =>
+          IO.print "d "
+          IO.print <| delLine.clauses.foldl (fun str clause => str ++ s!"{clause + 1} ") ""
+          IO.println "0"
+        loop index
+    else
+      return
+  loop 0
+
+partial def main : List String → IO Unit
+  | [] => printUsage
+  | filePath :: args => do
+    match args with
+    | [] => echoLSR filePath
+    | ["cnf"] => echoCnf filePath
+    | ["lsr"] => echoLSR filePath
+    | ["clsr"] => echoLSRBinary filePath
+    | _ => printUsage
