lakefile.lean
@@ -16,9 +16,30 @@ lean_lib Experiments {
   globs := #[.submodules `Experiments]
 }
 
+lean_exe «SRParser» {
+  root := `Experiments.ProofChecking.SRParserExe
+}
+
+lean_exe «SRChecker» {
+  root := `Experiments.ProofChecking.SRCheckerExe
+}
+
 lean_exe «FormulaParser» {
   root := `Experiments.ProofChecking.SRParser
 }
+
+lean_exe «SRCheckerEfficient» {
+  root := `Experiments.ProofChecking.SRParserEfficient
+}
+
+lean_exe «StatefulChecker» {
+  root := `Experiments.ProofChecking.SRParserStateful
+}
+
+lean_exe «BasicChecker» {
+  root := `Experiments.ProofChecking.SRCheckerBasic
+}
+
 
 -- Note: `mathlib` and `std` are obtained transitively so that the versions all match up
 require leancolls from git "https://github.com/JamesGallicchio/LeanColls.git" @ "v4.7.0"
